As mentioned in the last Skype call, the [Term] datatype of L1g, L1_5, L2 and L3 now containg a constructor [TWrong], and compiling no longer returns option or exception.  THIS WILL BREAK SOMETHING IN L4, which I haven't fixed.
I made lots of other changes.  The only other change I think may be
observable to other levels of the compiler is that wcbvEval of L3
(both the relation and the function versions) is slightly more
liberal.  This change should not be observable for terms that come
from Coq.  (This is a time dependent claim, as Coq might change, and
the arbitrary internal representation that template-coq represents may
change.)

Updating before this commit, I had a good deal of frustration fixing
conflicts introduced by Matthieu (and a minor one by Abhishek).  Every
file in L3 had a conflict.  I realize Matthieu changed template-coq,
which naturally propogates through the whole compiler, but making the
changes for myself would leave me in better mood than fixing conflicts
and merges that didn't work in many files.

In future PLEASE DON'T CHANGE MY FILES WITHOUT FIRST EMAILING ME ABOUT
IT!!!.  Remember I am currently responsible for languages L1g, L1_5,
L2 and L3, which is a lot of files for conflicts.

certicoq/theories/L1_5_box/awndEval.v
@@ -25,11 +25,11 @@ Set Implicit Arguments.
 
 (*** alrernative non-deterministic small step evaluation relation ***)
 Section Env.
-Variable p:environ.
+Variable p:environ Term.
 Inductive awndEval : Term -> Term -> Prop :=
 (** contraction steps **)
 | aConst: forall (s:string) (t:Term),
-         WFapp t -> LookupDfn s p t -> awndEval (TConst s) t
+         LookupDfn s p t -> awndEval (TConst s) t
 | aBeta: forall (nm:name) (ty bod arg:Term) (args:Terms),
            awndEval (TApp (TLambda nm ty bod) arg args)
                    (whBetaStep bod arg args)
@@ -81,31 +81,17 @@ Inductive awndEval : Term -> Term -> Prop :=
 | aCaseBrs: forall (ml:inductive * nat * list nat) (ty mch:Term) (brs brs':Terms),
               awndEvals brs brs' ->
               awndEval (TCase ml ty mch brs) (TCase ml ty mch brs')
-| aFixDefs: forall (ds es:Defs) (i:nat),
-              awndDEvals ds es -> awndEval (TFix ds i) (TFix es i)
 with awndEvals : Terms -> Terms -> Prop :=
      | aaHd: forall (t r:Term) (ts:Terms), 
                awndEval t r ->
                awndEvals (tcons t ts) (tcons r ts)
      | aaTl: forall (t:Term) (ts ss:Terms),
                awndEvals ts ss ->
-               awndEvals (tcons t ts) (tcons t ss)
-with awndDEvals : Defs -> Defs -> Prop :=
-     | adaHd: forall (n:name) (t r s:Term) (i:nat) (ds:Defs), 
-               awndEval t r ->
-               awndDEvals (dcons n t s i ds) (dcons n r s i ds)
-     | adaHd2: forall (n:name) (t r s:Term) (i:nat) (ds:Defs), 
-               awndEval t r ->
-               awndDEvals (dcons n s t i ds) (dcons n s r i ds)
-     | adaTl: forall (n:name) (t s:Term) (i:nat) (ds es:Defs),
-               awndDEvals ds es ->
-               awndDEvals (dcons n t s i ds) (dcons n t s i es).
-Hint Constructors awndEval awndEvals awndDEvals.
+               awndEvals (tcons t ts) (tcons t ss).
+Hint Constructors awndEval awndEvals.
 Scheme awndEval1_ind := Induction for awndEval Sort Prop
-     with awndEvals1_ind := Induction for awndEvals Sort Prop
-     with awndDEvals1_ind := Induction for awndDEvals Sort Prop.
-Combined Scheme awndEvalEvals_ind
-         from awndEval1_ind, awndEvals1_ind, awndDEvals1_ind.
+     with awndEvals1_ind := Induction for awndEvals Sort Prop.
+Combined Scheme awndEvalEvals_ind from awndEval1_ind, awndEvals1_ind.
 
 Definition no_awnd_step (t:Term) : Prop :=
   no_step awndEval t.
@@ -159,12 +145,15 @@ Lemma awndEval_Cast_inv:
 Qed.
 
 Lemma awndEval_pres_WFapp:
+  WFaEnv p ->
   (forall t s, awndEval t s -> WFapp t -> WFapp s) /\
-  (forall ts ss, awndEvals ts ss -> WFapps ts -> WFapps ss) /\
-  (forall ds es, awndDEvals ds es -> WFappDs ds -> WFappDs es) .
+  (forall ts ss, awndEvals ts ss -> WFapps ts -> WFapps ss).
 Proof.
+  intros hp.
   apply awndEvalEvals_ind; intros; try assumption;
   try (solve [inversion_Clear H0; constructor; intuition]).
+  - unfold LookupDfn in l. assert (j:= Lookup_pres_WFapp hp l).
+    inversion j. assumption.
   - inversion_Clear H. inversion_Clear H4.
     apply whBetaStep_pres_WFapp; assumption.
   - inversion_Clear H. apply instantiate_pres_WFapp; assumption.
@@ -202,19 +191,15 @@ Inductive awndEvalsRTC : Terms -> Terms -> Prop :=
 | awEsRTCstep: forall ts ss, awndEvals ts ss -> awndEvalsRTC ts ss
 | awEsRTCtrn: forall ts ss us,
        awndEvalsRTC ts ss -> awndEvalsRTC ss us -> awndEvalsRTC ts us.
-Inductive awndDEvalsRTC: Defs -> Defs -> Prop :=
-| awDEsRTCrfl: forall ts, awndDEvalsRTC ts ts
-| awDEsRTCstep: forall ts ss, awndDEvals ts ss -> awndDEvalsRTC ts ss
-| awDEsRTCtrn: forall ts ss us, awndDEvalsRTC ts ss -> awndDEvalsRTC ss us ->
-                          awndDEvalsRTC ts us.
-Hint Constructors awndEvalRTC awndEvalsRTC awndDEvalsRTC.
+Hint Constructors awndEvalRTC awndEvalsRTC.
 
 
 Lemma awndEvalRTC_pres_WFapp:
-  forall t s, awndEvalRTC t s -> WFapp t -> WFapp s.
+    WFaEnv p -> forall t s, awndEvalRTC t s -> WFapp t -> WFapp s.
 Proof.
+  intros hp.
   induction 1; intros; try assumption.
-  - eapply (proj1 (awndEval_pres_WFapp)); eassumption.
+  - eapply (proj1 (awndEval_pres_WFapp hp)); eassumption.
   - apply IHawndEvalRTC2; try assumption.
     + apply IHawndEvalRTC1; assumption.
 Qed.
@@ -234,13 +219,8 @@ Qed.
 
 
 End Env.
-Hint Constructors awndEval awndDEvals awndEvals.
-Hint Constructors awndEvalRTC awndEvalsRTC awndDEvalsRTC.
-(***
-Hint Constructors awndEvalTC awndEvalsTC.
-Hint Constructors awndEvalTCl awndEvalsTCl.
-***)
-
+Hint Constructors awndEval awndEvals.
+Hint Constructors awndEvalRTC awndEvalsRTC.
 
 
 (**
